Add problem to ps1

ps/ps1_fundamentals.dfy
@@ -6,6 +6,7 @@
 
 // Write a stronger precondition for this method
 // Hint: The range of a also applies to b
+
 method MaxProduct(a: int, b: int) returns (max: int, pro: int)
     requires 0 <= a <= 100 // Edit this line only
     ensures pro == a * b 
@@ -18,4 +19,49 @@ method MaxProduct(a: int, b: int) returns (max: int, pro: int)
         max := b;
     }
     pro := a * b;
+}
+
+
+// Problem 2
+
+// Whereas methods are opaque, functions are transparant.
+// Hence, they can be used in specifications.
+
+// Predicate is a form of function that only returns boolean value
+
+// A construct (function, variable, etc) that is used only for
+// verification and not required at compile-time is called "ghost"
+
+// We can label constructs as "ghost" to make it explicit.
+// For example,
+
+// ghost function Square(x: int): int {
+//     x * x
+// }
+
+// Label all declarations in the code below that are not
+// required at compile-time as ghost.
+
+// Hint: A ghost is not allowed on right side of assignment
+// Hint: There are 5 ghosts in total
+
+predicate IsEven(x: int) {
+    x % 2 == 0
+}
+
+predicate IsOdd(x: int) {
+    x % 2 != 0
+}
+
+method SomeMethod(x: nat, y: nat) returns (r: int)
+    requires IsEven(x) || IsOdd(y)
+    requires x + y < 100
+    ensures (x % 5 == 0 && y % 5 == 0) ==> r == x + y
+    ensures (x % 5 != 0 || y % 5 != 0) ==> r == x - y
+{
+    if x % 5 == 0 && y % 5 == 0 {
+        r := x + y;
+    } else {
+        r := x - y;
+    }
 }
